abstract algorithm for VC to SC

TSTSC_Poly.thy
@@ -153,6 +153,8 @@ subsection \<open>A trivial implementation\<close>
 text \<open>Here we assume that we have an operation that returns
       the size of the set of vertices.\<close>
 
+definition "mop_get_vertices E = REST [ (\<Union> E)  \<mapsto> 2 * card E + 1]"
+
 definition "mop_get_vertices_card E = REST [(card (\<Union> E)) \<mapsto> 2 * card E + 2]"
 
 text \<open>Then we can easily give an abstract algorithm for the reduction:\<close>
@@ -247,9 +249,11 @@ qed
 
 text \<open>now let's implement getting the cardinality of V with the basic set operations\<close>
 
-definition get_vertices_card :: "('b*'b) list \<Rightarrow> nat nrest" where
-  "get_vertices_card es = do {
-      S \<leftarrow> mop_set_empty_set;
+definition "mop_get_vertices' es = SPECT [\<Union> ((\<lambda>(a,b). {a,b}) ` (set es)) \<mapsto> 2 * length es + 1]"
+
+definition get_vertices where
+  "get_vertices es = 
+    do { S \<leftarrow> mop_set_empty_set;
       S' \<leftarrow> nfoldli es (\<lambda>_. True) 
             (\<lambda>(a,b) S. do {
                   S \<leftarrow> mop_set_insert S a;
@@ -257,18 +261,17 @@ definition get_vertices_card :: "('b*'b) list \<Rightarrow> nat nrest" where
                   RETURNT S }) 
 
         S;
-      n \<leftarrow> mop_set_card S';
-      RETURNT n
-    }"
- 
+      RETURNT S' 
+  }"
 
-lemma get_vertices_card_refine:
-  "get_vertices_card xs \<le> mop_get_vertices_card' xs"
+
+lemma get_vertices_refine:
+  "get_vertices xs \<le> mop_get_vertices' xs"
 proof -
   let ?I = "\<lambda>(xs::('b*'b)list) ys (S::'b set).  S = \<Union> ((\<lambda>(a,b). {a,b}) ` (set xs))"
 
   show ?thesis
-  unfolding get_vertices_card_def mop_get_vertices_card'_def
+  unfolding get_vertices_def mop_get_vertices'_def
   apply(rule T_specifies_I)
   apply(subst nfoldliIE_def[symmetric, where I="?I" and E=2])
   unfolding mop_set_empty_set_def
@@ -289,6 +292,27 @@ proof -
    apply (auto simp add: one_enat_def)    
   done 
 qed
+
+definition get_vertices_card :: "('b*'b) list \<Rightarrow> nat nrest" where
+  "get_vertices_card es = do {
+      V \<leftarrow> get_vertices es;
+      n \<leftarrow> mop_set_card V;
+      RETURNT n
+    }"
+ 
+thm get_vertices_refine[unfolded mop_get_vertices'_def,
+                THEN T_specifies_rev, THEN T_conseq4]
+
+lemma get_vertices_card_refine:
+  "get_vertices_card xs \<le> mop_get_vertices_card' xs" 
+  unfolding get_vertices_card_def mop_get_vertices_card'_def
+  apply(rule T_specifies_I) 
+  apply(vcg' - rules: get_vertices_refine[unfolded mop_get_vertices'_def,
+                THEN T_specifies_rev, THEN T_conseq4]) 
+  unfolding mop_set_card_def
+  apply (vcg' -) unfolding Some_le_emb'_conv Some_eq_emb'_conv
+  by (auto simp add: one_enat_def split: if_splits)    
+ 
 
 lemma get_vertices_card_data_refine:
   assumes "(xs,E)\<in>R_edge_set_tuple_list"
@@ -348,6 +372,234 @@ lemma "ispolyredd is_to_vc2
   apply(rule is_to_vc2_refines' ) .
 
 
+section "VC to SC"
+
+
+definition "mop_set_to_list V = SPEC (\<lambda>xs. set xs = V \<and> distinct xs) (\<lambda>_. 1)"
+
+definition "mop_set_member S s = SPECT [ s \<in> S \<mapsto> 1] "
+
+definition "mop_check_ugraph E = SPECT [ugraph E \<mapsto> 1]"
+
+
+definition "innerset = (\<lambda>v es.
+ do {
+  Rv \<leftarrow> mop_set_empty_set;
+  Rv \<leftarrow> nfoldli es (\<lambda>_. True)
+          (\<lambda>e Rv. do { 
+                    b \<leftarrow> mop_set_member e v;
+                    if b then mop_set_insert Rv e
+                       else RETURNT Rv})
+      Rv;
+  RETURNT Rv
+})"
+
+definition "innerset_spec v es = SPECT [  {e. e \<in> (set es) \<and> v \<in> e} \<mapsto> (1+1) * length es + 1 ]"
+
+lemma innerset_refines:
+  "innerset v es \<le> innerset_spec v es"
+proof -
+  let ?I="\<lambda>xs ys S. S = {e. e \<in> set xs \<and> v \<in> e} "
+
+  show ?thesis
+    unfolding innerset_def innerset_spec_def  mop_set_empty_set_def mop_set_member_def mop_set_insert_def
+    apply(subst nfoldliIE_def[symmetric, where I="?I" and E="2"])
+    apply(rule T_specifies_I)
+    apply(vcg' \<open>-\<close> rules: T_SPEC )
+    unfolding mop_set_empty_set_def
+    apply(vcg' -) 
+    apply(rule nfoldliIE_rule[THEN T_specifies_rev, THEN T_conseq4, where P2="?I es []" ])
+    subgoal apply simp done
+    subgoal unfolding mop_set_insert_def
+      apply(rule T_specifies_I)
+      apply(vcg' \<open>-\<close> rules:  ) unfolding Some_le_emb'_conv Some_eq_emb'_conv
+      by (auto simp add: one_enat_def split: if_splits)    
+    subgoal by auto 
+    subgoal by auto 
+     apply (rule order.refl) 
+    subgoal apply(vcg' -) unfolding Some_le_emb'_conv Some_eq_emb'_conv
+      by (auto simp add: one_enat_def split: if_splits) 
+    done
+qed
+
+definition "outerset = (\<lambda>es vs.
+  do {
+    R \<leftarrow> mop_set_empty_set;
+    R \<leftarrow> nfoldli vs (\<lambda>_. True)
+       (\<lambda>v R. do {
+              Rv \<leftarrow> innerset v es;
+              R \<leftarrow> mop_set_insert R Rv;
+               RETURNT R })
+         R;
+    RETURNT R
+  })" 
+
+definition "outerset_spec es vs
+       = SPECT [  {{e. e \<in> set es \<and> v \<in> e} | v. v \<in> set vs} \<mapsto> 1 + ( 2 + (1+1) * length es) * length vs]"
+
+lemmas aha = innerset_refines[unfolded innerset_spec_def,
+                THEN T_specifies_rev, THEN T_conseq4]
+
+lemma outerset_refines:
+  "outerset es vs \<le> outerset_spec es vs"
+proof -
+  let ?I="\<lambda>xs ys S. S = {{e. e \<in> set es \<and> v \<in> e} | v. v \<in> set xs} "
+
+  show ?thesis
+    unfolding outerset_def outerset_spec_def  mop_set_empty_set_def
+    apply(subst nfoldliIE_def[symmetric, where I="?I" and E="2*length es + 2"])
+    apply(rule T_specifies_I)
+    apply(vcg' \<open>-\<close> rules: T_SPEC )
+    unfolding mop_set_empty_set_def
+    apply(vcg' -) 
+    apply(rule nfoldliIE_rule[THEN T_specifies_rev, THEN T_conseq4, where P2="?I vs []" ])
+    subgoal apply simp done
+    subgoal unfolding mop_set_insert_def
+      apply(rule T_specifies_I)
+      apply(vcg' \<open>-\<close> rules: aha) unfolding Some_le_emb'_conv Some_eq_emb'_conv
+      by (auto simp add: one_enat_def split: if_splits)    
+    subgoal by auto 
+    subgoal by auto 
+     apply (rule order.refl) 
+    subgoal apply(vcg' -) unfolding Some_le_emb'_conv Some_eq_emb'_conv
+      by (auto simp add: one_enat_def split: if_splits) 
+    done
+qed
+
+
+definition "vc_to_sc = (\<lambda>(E,k).   
+  do {
+    b \<leftarrow> mop_check_ugraph E;
+    V  \<leftarrow> mop_get_vertices E;
+    cV \<leftarrow> mop_set_card V;
+    vs \<leftarrow> mop_set_to_list V;
+    if b \<and> k \<le> cV then
+      do {
+        es \<leftarrow> mop_set_to_list E;
+        ASSERT (length vs \<le> 2 * length es);
+        ASSERT (length es = card E);
+        R \<leftarrow> outerset es vs;
+        RETURNT ( R, k)
+      }
+    else RETURNT ( {{undefined}}, 0 )
+  } )"
+
+
+
+definition "sc_time n = 1+1+ (2 * n + 1) + 1 + 1 + (1 + ( 1 + (1+1) * n) * (4*n))" 
+
+
+lemmas aha2 = outerset_refines[unfolded outerset_spec_def,
+                THEN T_specifies_rev, THEN T_conseq4]
+
+lemma pf: "a\<le>b \<Longrightarrow> enat a \<le> enat b" by auto 
+lemma k: "enat a + enat b = enat (a+b)" by auto
+ 
+
+lemma card_Un: "finite E \<Longrightarrow> card (\<Union>E) \<le> sum card E"
+  by(induct  rule: finite_induct) (auto intro: order.trans[OF card_Un_le]) 
+
+lemma vc_to_sc_refines:
+  "vc_to_sc (E,k) \<le> SPEC (\<lambda>y. y = vc_sc (E,k)) (\<lambda>_. sc_time (size_VC (E,k)))"
+  unfolding SPEC_def
+  unfolding vc_to_sc_def vc_sc_def   
+      mop_set_to_list_def mop_get_vertices_def mop_set_card_def
+      mop_check_ugraph_def
+  apply(rule T_specifies_I)
+  apply(vcg' \<open>-\<close> rules: T_SPEC aha2)
+  subgoal apply simp  apply safe
+       apply(auto split: if_splits) 
+    subgoal premises prems apply(auto simp: sc_time_def size_VC_def)
+      unfolding one_enat_def apply simp
+      apply(rule add_mono)   
+      subgoal using prems(8,9) by auto
+      subgoal using prems(8,9) apply(intro mult_mono) by auto
+      done
+    done 
+  subgoal
+    by(auto simp: distinct_card)
+  subgoal    for a b x xa
+    unfolding ugraph_def apply auto
+    subgoal premises prems
+    proof -
+      have "length x = card (\<Union> a)" 
+        apply(subst distinct_card[symmetric])
+        using prems  by auto
+      also have "\<dots> \<le> sum card a"
+        apply(rule card_Un) using prems by simp
+      also have "\<dots> = sum card (set xa)" using prems by auto
+      also have "\<dots> = 2 * card (set xa)" using prems by simp
+      also have "\<dots> = 2 * length xa" 
+        apply(subst distinct_card[symmetric])using prems by auto
+      finally show ?thesis .
+    qed
+    done
+  subgoal
+    apply auto
+    unfolding Some_le_emb'_conv Some_eq_emb'_conv
+    by (auto simp: size_IS_def size_VC_def sc_time_def  one_enat_def) 
+  done
+
+
+
+definition "size_SC = (\<lambda>(E,k). sum card E)"
+
+definition "sc_space n = 1 + 2 * (n * n)" 
+  
+
+lemma sum_Un: "finite E \<Longrightarrow> (\<And>e. e\<in>E \<Longrightarrow> finite e) \<Longrightarrow> (\<And>x. f x \<ge> (0::nat))
+     \<Longrightarrow> sum f (\<Union>E) \<le> sum (\<lambda>x. sum f x) E"
+  by (induct  rule: finite_induct) 
+    (simp_all add: sum_Un_nat) 
+
+
+lemma vc_to_sc_size:
+  "size_SC (vc_sc a) \<le> sc_space (size_VC a)"
+  apply(cases a)
+  apply (auto simp: vc_sc_def size_SC_def size_VC_def vc_time_def sc_space_def)
+  subgoal premises prems for E k
+  proof -
+    have *: "{{e \<in> E. v \<in> e} |v. \<exists>x\<in>E. v \<in> x} = (\<lambda>v. {e \<in> E. v \<in> e}) ` (\<Union> E)" by blast
+    have "sum card {{e \<in> E. v \<in> e} |v. \<exists>x\<in>E. v \<in> x}
+      = sum card ((\<lambda>v. {e \<in> E. v \<in> e}) ` (\<Union> E))" unfolding * ..
+    also have "\<dots> \<le> sum (card o (\<lambda>v. {e \<in> E. v \<in> e})) (\<Union> E)"
+      apply(rule sum_image_le) using prems(2) ugraph_vertex_set_finite by auto
+    also have "\<dots> \<le> sum (\<lambda>x. sum (card o (\<lambda>v. {e \<in> E. v \<in> e})) x) E " apply(rule sum_Un)
+      using prems unfolding ugraph_def apply auto  
+      by (meson finite_subset le_cSup_finite prems(2) ugraph_vertex_set_finite)  
+    also have "\<dots> \<le> sum (\<lambda>x. sum (\<lambda>_. card E) x) E"
+      apply(rule sum_mono)
+      apply(rule sum_mono) apply auto  
+      by (metis (no_types, lifting) card_mono mem_Collect_eq prems(2) subsetI ugraph_def)   
+    also have "\<dots> = sum (\<lambda>x. 2 * card E) E" 
+      apply(rule sum.cong) using prems(2) unfolding ugraph_def by simp_all
+    also have "\<dots> = 2* (card E) * (card E)" by simp
+    finally show ?thesis by simp
+  qed
+  done
+
+
+lemma vc_to_sc_ispolyred: "ispolyred vc_to_sc vertex_cover set_cover size_VC size_SC" 
+  unfolding ispolyred_def
+  apply(rule exI[where x=vc_sc])
+  apply(rule exI[where x=sc_time])
+  apply(rule exI[where x=sc_space])
+  apply(safe)
+  subgoal using vc_to_sc_refines by blast
+  subgoal using vc_to_sc_size  by blast 
+  subgoal unfolding poly_def sc_time_def apply(rule exI[where x=2]) by auto
+  subgoal unfolding poly_def sc_space_def apply(rule exI[where x=2]) by auto
+  subgoal using is_reduction_vc_sc .
+  done
+
+
+
+
+
+section \<open>combination\<close>
+
+
+thm is_to_vc_ispolyred vc_to_sc_ispolyred  ispolyred_trans[OF is_to_vc_ispolyred vc_to_sc_ispolyred ]
 
 
 end
